
\section{Representation of the Brownian meander with drift}

For the non-drifted meander $ M(t), t>0 $ it is well known that the following representation holds
\begin{equation}\label{eq:mdr-repr}
\frac{
\Big|  B(T_0 + s (t - T_0)) \Big|
}{\sqrt{t - T_0}}
\stackrel{i.d.}{=} M(s) \qquad 0 < s < 1
\end{equation}
%
%
where $ T_0 =  \sup\{  s < t : B(s) = 0\} $ and $ B(t), t>0  $  is a standard Brownian motion (see \citet{pitman99}).

For the Brownian meander with drift we have instead the following result.

\begin{theorem}
	\begin{align}\label{eq:mdr-repr-thm}
	P\left\{   
	\frac { 
	\Big | B^\mu\Big ( T_0^\mu + s ( t - T_0^\mu) \Big )  \Big |    
	}
	{
	\sqrt{t - T^\mu_0}
	} \in \mathrm d y 
	\right\} = 
	\frac 12 
	\left[
	P\left\{ M^{- \mu \sqrt{ t - T_0^\mu}}(s) \in\mathrm d y \right\} + 
	P\left\{ M^{\mu \sqrt{ t - T_0^\mu}} (s)\in\mathrm d y \right\}  
	\right]
	\end{align}
for $  0< s < 1 $, where $ T_0^\mu $ is the last passage time through zero before $ t $ of $ B^\mu $ and has distribution
%
%
\begin{align*}
P( T _0^\mu \in \mathrm d a) / \mathrm d a &=
\frac{e^{- \frac{\mu^2 t }{2}}}{\pi \sqrt{a (t-a)}} + \frac{\mu^2}{2 \pi} \int_a^t \frac{e^{ - \frac{ \mu^2 a }{2 }}}{\sqrt{a ( y -a )}} 
\, \mathrm d y 
\numberthis 
\\
&=
\mathbb E \left( \frac{1 }{\pi \sqrt{a ( W -a )}} \mathds{1}_{W \geq a } \right) \qquad 0 <a<t
\end{align*}
where $  W  $ is a truncated exponential distribution with density
\begin{align*}
&f_W(w) = \frac{\mu^2}{2} e^{  - \frac{\mu^2}{2} w  } \qquad 0<w<t \\
&P(W = t ) = e^{-\frac{\mu^2 t}{2}}\, .
\end{align*}
\end{theorem}
%
%
\begin{proof}
	We start by observing that, for $  0< s<1 $
	\begin{align}
		P\left\{   
	\frac { 
		\Big | B^\mu\Big ( T_0^\mu + s ( t - T_0^\mu) \Big )  \Big |    
	}
	{
		\sqrt{t - T^\mu_0}
	} <  y 
	\right\} 
	= 
	\int_0^t P\left\{T_0^\mu \in \mathrm d z \right\} \int_{ -y \sqrt{t-z}}^{ y \sqrt{t-z}}
	P \left\{ 
	 B^\mu  ( T_0^\mu + s ( t - T_0^\mu) )  \in \mathrm d w \Big | T_0^\mu = z
	\right\}
	\end{align}
	and thus 
	\begin{align*}
	&
	P\left\{   
	\frac { 
		\Big | B^\mu\Big ( T_0^\mu + s ( t - T_0^\mu) \Big )  \Big |    
	}
	{
		\sqrt{t - T^\mu_0}
	} \in \mathrm d y 
	\right\} 
	\numberthis 
	\label{eq:mdr-repr-full}
	\\
	 &=
	 \int_0^t P\left\{T_0^\mu \in \mathrm d z \right\} \sqrt{t -z}
	 \big[
	 P \left\{ 
	 B^\mu ( z + s (t-z)) \in \mathrm d (  y \sqrt{t-z}) | T_0^\mu = z
 	 \right\} 
 	 \\
 	 & \qquad 
 	 +
 	 P \left\{ 
 	 B^\mu ( z + s (t-z)) \in \mathrm d ( - y \sqrt{t-z}) | T_0^\mu = z
 	 \right\} 
	 \big]
	\end{align*}
	%
	%
	Note that 
	\begin{align*}
	&
	P\left\{ 
	B^\mu ( z + s (t-z)) \in \mathrm d y \Big | (T_0^\mu = z) \cap 
	\Big ( 
	\big( 
	\inf_{z < l \leq t} B^\mu ( l ) > 0 
	 \big)
	 \cup 
	 \big( 
	 \sup_{z < l \leq t} B^\mu ( l ) < 0 
	 \big)
	 \Big)
	\right\}
	\numberthis 
	\\
	&=
	P\left\{ 
	B^\mu ( z + s (t-z)) \in \mathrm d y | (T_0^\mu = z) \cap 
	(C
	\cup 
	D)
	\right\}
	\\
	&=
	P\left\{ 
	B^\mu ( z + s (t-z)) \in \mathrm d y | (B^\mu(z) = 0) \cap 
	C
	\right\} 
	\frac{\displaystyle
		P(C | B^\mu(z) = 0 )}
	{
		\displaystyle
			P(C | B^\mu(z) = 0 )) + 
		P(D | B^\mu(z) = 0 ))}
	\\
	& 
	\qquad + 
	P\left\{ 
	B^\mu ( z + s (t-z)) \in \mathrm d y | (B^\mu(z) = 0) \cap 
	D
	\right\} 
	\frac{\displaystyle
		P(D | B^\mu(z) = 0 )}
	{
		\displaystyle
		P(C | B^\mu(z) = 0 )) + 
		P(D | B^\mu(z) = 0 ))}
	\end{align*}
	The ratio 
	$  \frac{P(D | B^\mu(z) = 0)}{P( C |B^\mu(z) = 0 )} $
	can be evaluated as the following limit
	\begin{align*}
	\frac{P(D | B^\mu(z) = 0)}{P( C |B^\mu(z) = 0 )} 
	&= 
	\lim_{u \downarrow 0 } 
	\frac{
		P ( \max_{z \leq l \leq t} B^\mu ( l ) < 0  | B^\mu(z) =  - u)
	}{P ( \min_{z \leq l \leq t} B^\mu ( l ) > 0  | B^\mu(z) =  u)}
	\\
	&=
	\lim_{u \downarrow 0 } 
	\frac{
		P ( \max_{0 \leq l \leq t - z } B^\mu ( l ) < 0  | B^\mu(0) =  - u)
	}{P ( \min_{0 \leq l \leq t -z } B^\mu ( l ) > 0  | B^\mu(0) =  u)}
	\\
	&=
	\lim_{u \downarrow 0 } 
	\frac{
		P ( \overline T_0^\mu > t -z   | B^\mu(0) =  - u)
	}{P ( \overline T_0^\mu > t -z   | B^\mu(0) =  u)}
	\\
	&=
	\lim_{u \downarrow 0 } 
	\frac{
		1 - \int_0^{t-z} 
		u \, \frac{
		e^{ - \frac{ (u - \mu s ) ^ 2 }{2 s } }	
	}{\sqrt{2 \pi s^3}} \, \mathrm d s
	}{
	1 - \int_0^{t-z} 
	u \, \frac{
		e^{ - \frac{ (u + \mu s ) ^ 2 }{2 s } }	
	}{\sqrt{2 \pi s^3}} \, \mathrm d s
	}
	=
	1 
	\end{align*}
	where
	$  \overline T _ 0 ^ \mu = \inf\{ s : B^\mu(s) = 0\} $ is the first passage time of a drifted 
	Brownian motion starting either above or below zero. 
	
	In view of formula \eqref{eq:bmd-drift-dist-prooved}, for $  v = 0, s = l - z, t $ replaced by $  t -z  $
	we obtain, by setting $  l = z + s ( t-z) $ that
	\begin{align*}
	&
	P\left\{ 
	B^\mu ( l) \in \mathrm d y | B^\mu(z)  = 0 ,  
	\inf_{z < w \leq t} B^\mu ( w ) > 0 
	\right\}
	\numberthis 
	\label{eq:mdr-repr-min}
	\\
	&=
	P\left\{ 
	B^\mu ( l - z ) \in \mathrm d y | B^\mu(z)  = 0 ,  
	\inf_{0 < w \leq t - z } B^\mu ( 0 ) > 0 
	\right\}
	\\
	&=
	\left ( \frac{t - z  }{l - z }\right ) ^{\!\frac 32}
	\frac{
		\mathrm d y \,\, 
		y e^{ - \frac{ y^2}{2 (l-z) }} 		
	}{
		%
		\int_0^\infty 
		w 
		%
		e^{- \frac{ w^2}{2 (t-z)}  + \mu w}    
		\, \mathrm d w 		
	}\,
	\int_0^\infty 
	\Big( 
	e^{- \frac{ ( w - y)^2}{2(t-l)}} 
	- e^{   - \frac{ (w+y)^2}{2 ( t-l)}   }
	\Big ) 
	\frac{  e^{ \mu w } } {\sqrt{2 \pi (t - l)}}
	 \, \mathrm d w
	\end{align*}
	%
	In the same way we have that
	\begin{align*}
	&
	P\left\{ 
	B^\mu ( l) \in \mathrm d y | B^\mu(z)  = 0 ,  
	\sup_{z < w \leq t} B^\mu ( w ) < 0 
	\right\}
	\numberthis 
	\label{eq:mdr-repr-max}
	\\
	&=
	\left ( \frac{t - z  }{l - z }\right ) ^{\!\frac 32}
	\frac{
		\mathrm d y \,\, 
		y e^{ - \frac{ y^2}{2 (l-z) }} 		
	}{
		%
		\int_0^\infty 
		w 
		%
		e^{- \frac{ w^2}{2 (t-z)}  - \mu w}    
		\, \mathrm d w 		
	}\,
	\int_0^\infty 
	\Big( 
	e^{- \frac{ ( w - y)^2}{2(t-l)}} 
	- e^{   - \frac{ (w+y)^2}{2 ( t-l)}   }
	\Big ) 
	\frac{  e^{ - \mu w } } {\sqrt{2 \pi (t - l)}}
	\, \mathrm d w
	\end{align*}
	%
	%
	By inserting  \eqref{eq:mdr-repr-min} and  \eqref{eq:mdr-repr-max} 
	into \eqref{eq:mdr-repr-full}  we obtain 
	\begin{align*}
	&
	P\left\{   
	\frac { 
		\Big | B^\mu\Big ( T_0^\mu + s ( t - T_0^\mu) \Big )  \Big |    
	}
	{
		\sqrt{t - T^\mu_0}
	} \in \mathrm d y 
	\right\} 
	=
	\frac{1}{2}
	\int_0^t P \{ T_0^\mu \in \mathrm d z \}  \quad \times
	\numberthis 
	\label{eq:mdr-repr-full-ins}
	\\
	& \qquad \times 
	\Bigg[ 
	 \frac{1}{s^{\!\frac 32} } 
	\frac{
		\mathrm d y \,\, 
		y \sqrt{t-z} \, e^{ - \frac{ y^2}{2 s }} 		
	}{
		%
		\int_0^\infty 
		w 
		%
		e^{- \frac{ w^2}{2 (t-z)}  + \mu w}    
		\, \mathrm d w 		
	}\,
	\int_0^\infty 
	\Big( 
	e^{- \frac{ ( w - y \sqrt{t-z}   )^2  }{    2(t-z)(1-s)}} 
	- e^{   - \frac{ (w+y \sqrt{t-z} )^2}{2 ( t-z)(1-s)}   }
	\Big ) 
	\frac{  e^{ \mu w } } {\sqrt{2 \pi (1-s)}}
	\, \mathrm d w 
	\\
	& \qquad \hphantom{\Bigg[  }  + 
	\frac{1}{s^{\!\frac 32} } 
	\frac{
		\mathrm d y \,\, 
		y \sqrt{t-z} \, e^{ - \frac{ y^2}{2 s }} 		
	}{
		%
		\int_0^\infty 
		w 
		%
		e^{- \frac{ w^2}{2 (t-z)}  - \mu w}    
		\, \mathrm d w 		
	}\,
	\int_0^\infty 
	\Big( 
	e^{- \frac{ ( w - y \sqrt{t-z}   )^2  }{    2(t-z)(1-s)}} 
	- e^{   - \frac{ (w+y \sqrt{t-z} )^2}{2 ( t-z)(1-s)}   }
	\Big ) 
	\frac{  e^{ - \mu w } } {\sqrt{2 \pi (1-s)}}
	\, \mathrm d w
	\Bigg] 
	\end{align*}
	%
	%
	The transformation $ w = w' \sqrt{t-z} $ further simplifies \eqref{eq:mdr-repr-full-ins}
	as
	\begin{align*}
	&
	P\left\{   
	\frac { 
		\Big | B^\mu\Big ( T_0^\mu + s ( t - T_0^\mu) \Big )  \Big |    
	}
	{
		\sqrt{t - T^\mu_0}
	} \in \mathrm d y 
	\right\} 
	=
	\frac{1}{2}
	\int_0^t P \{ T_0^\mu \in \mathrm d z \}  \quad \times
	\numberthis 
	\label{eq:mdr-repr-full-ins-2}
	\\
	& \qquad \times 
	\Bigg[ 
	\frac{
		\mathrm d y \,\, 
		s^{ -\frac 32}
		y \, e^{ - \frac{ y^2}{2 s }} 		
	}{
		%
		\int_0^\infty 
		w 
		%
		e^{- \frac{ w^2}{2}  + \mu w\sqrt{t-z}}    
		\, \mathrm d w 		
	}\,
	\int_0^\infty 
	\Big( 
	e^{- \frac{ ( w - y    )^2  }{    2(1-s)}} 
	- e^{   - \frac{ (w+y  )^2}{2 (1-s)}   }
	\Big ) 
	\frac{  e^{ \mu w \sqrt{t-z}} } {\sqrt{2 \pi (1-s)}}
	\, \mathrm d w 
	\\
	& \qquad \hphantom{\Bigg[  }  + 
	\frac{
		\mathrm d y \,\, 
		s^{ -\frac 32}
		y \, e^{ - \frac{ y^2}{2 s }} 		
	}{
		%
		\int_0^\infty 
		w 
		%
		e^{- \frac{ w^2}{2 }  - \mu w\sqrt{t-z}}    
		\, \mathrm d w 		
	}\,
	\int_0^\infty 
	\Big( 
	e^{- \frac{ ( w - y   )^2  }{    2(1-s)}} 
	- e^{   - \frac{ (w+y  )^2}{2 (1-s)}   }
	\Big ) 
	\frac{  e^{ - \mu w \sqrt{t-z} } } {\sqrt{2 \pi (1-s)}}
	\, \mathrm d w
	\Bigg] 
	\end{align*}
	We recognize  inside \eqref{eq:mdr-repr-full-ins-2} the distribution of a drifted Brownian meander
	whose drift can be written as 
	\[
	\mu X \sqrt{t - T^\mu_0} 
	\]
	where $ X $ is a two-valued, symmetric r.v. independent from $ T^\mu_0  $ which is 
	the last-passage time through zero, before $ t $, of  the Brownian motion $ B^\mu $. 
	In conclusion we have that 
	\begin{align*}
	P\left\{   
	\frac { 
		\Big | B^\mu\Big ( T_0^\mu + s ( t - T_0^\mu) \Big )  \Big |    
	}
	{
		\sqrt{t - T^\mu_0}
	} \in \mathrm d y 
	\right\} 
	=
	%
	P\left\{ 
	M^{\mu X \sqrt{t - T^\mu_0} } ( s) \in \mathrm d y
	\right\}
	\end{align*}
\end{proof}
%
%
%
%%
%
\begin{remark}
	For $ \mu = 0 $ result \eqref{eq:mdr-repr-thm} coincides with \eqref{eq:mdr-repr}, valid 
	for the non-drifted Brownian meander.
\end{remark}














% !TeX root = ./mdr-main.tex