%
\section{About the maximum of the Brownian meander}
%
%
%
In this section we study the distribution of the maximum of the drifted Brownian meander and then we use the results about the maximum to derive the distribution of the first passage time.
\subsection{Maximum.}
As far as the maximum is concerned we have that for $ s<t, x>v, x>u $, 
%
\begin{align*}
&
P\bigg\{ \max_{0 \leq z \leq s} B^\mu(z) <x \Big |  \min_{0 \leq z \leq t} B^\mu (z) > v, B^\mu(0) = u  \bigg\}
\numberthis 
\label{eq:max-bmd-ini}
\\
&=
\int_v^x 
P \bigg\{  v < \min_{0 \leq z \leq s} B^\mu(z) < \max_{0 \leq z \leq s} B^\mu(z) < x , 
	B^\mu(s) \in  \mathrm d y
	\Big | 
	B^\mu(0) = u
	 \bigg\} \times 
 	\\
 	& \qquad 
 	\times 
 	\frac{
 		P\Big\{   \min_{s \leq z \leq t} B^\mu(z)   > v  \Big | B^\mu ( s) = y \Big\}
 	}{
 		P\Big\{   \min_{0 \leq z \leq t} B^\mu(z)   > v  \Big | B^\mu ( 0) = u \Big\}
	}
	\\
	%
	%
	%
	&=
	\int_v^x \, \frac{\mathrm d y}{\sqrt{2 \pi s}} \sum_{k = - \infty}^{+\infty}
	\left[ 
	%
	e^{    -   \frac{(y - u - 2k(x-v))^2}{2s} } 
	- 
	%
	e^{    -   \frac{(2v - y - u +2k(x-v))^2}{2s} }  
	\right ] 
	e^{ - \frac{\mu^2s}{2} + \mu ( y - u - 2k(x-v))} 
	\,\,\times 
	\\
	& \qquad \times 
	%
	\frac{
		P\Big\{   \min_{s \leq z \leq t} B^\mu(z)   > v  \Big | B^\mu ( s) = y \Big\}
	}{
		\int_v^\infty 
		\left[ 
		% 
		e^{  - \frac{(y-u)^2}{2t}  } 
		- 
		%
		e^{  - \frac{(2v - y-u)^2}{2t}  } 
		\right]
		e^{  - \frac{\mu^2 t}{2} + \mu ( y - u)   } \, \frac{ \mathrm d y}{\sqrt{2 \pi t} } 
	} \, \, .
\end{align*}
%
%
%
A certain simplification is obtained by letting $  s \to t $ and formula 
\eqref{eq:max-bmd-ini}  becomes
%
%
%
\begin{align*}
	&
	P\bigg\{ \max_{0 \leq z \leq t} B^\mu(z) <x \Big |  \min_{0 \leq z \leq t} B^\mu (z) > v, B^\mu(0) = u  \bigg\}
	\numberthis 
	\label{eq:max-bmd-t}
	\\
	&=
	\frac{
		\int_v^x \sum_{k = - \infty}^{+\infty}
		\left[ 
		%
			e^{    -   \frac{(y - u - 2k(x-v))^2}{2t} } 
		- 
		%
			e^{    -   \frac{(2v - y - u +2k(x-v))^2}{2t} }  %
		\right ] 
		e^{ - \frac{\mu^2t}{2} + \mu ( y - u - 2k(x-v))}
		\, \frac{ \mathrm d y}{\sqrt{2 \pi t} }
	}{
		\int_v^\infty 
		\left[ 
		%
			e^{  - \frac{(y-u)^2}{2t}  }  
		- 
		%
			e^{  - \frac{(2v - y-u)^2}{2t}  } 
		\right]
		e^{  - \frac{\mu^2 t}{2} + \mu ( y - u)   } \, \frac{ \mathrm d y}{\sqrt{2 \pi t} }
	} \, \, .
\end{align*}
%
%
Formula \eqref{eq:max-bmd-ini} for $  u \downarrow v $ yields
%
%
\begin{align*}
	&
	P\bigg\{ \max_{0 \leq z \leq s} B^\mu(z)<x \Big |  \inf_{0 < z < t} B^\mu (z) > v, B^\mu(0) = v  \bigg\}
	\numberthis 
	\label{eq:max-bmd-v}
	\\
	&=
		\int_v^x \sum_{k = - \infty}^{+\infty}
		%
			e^{    -   \frac{(y - v - 2k(x-v))^2}{2 s} } 
		\frac { (y - v - 2k (x-v) )}{s\sqrt{2 \pi s}}
		e^{ - \frac{\mu^2 s}{2} + \mu ( y - v- 2k(x-v))}
		\, \times 
		\\
		& \qquad \times 
		\frac{ 
		P\Big\{   \min_{s \leq z \leq t} B^\mu(z)   > v  \Big | B^\mu ( s) = y \Big\}
		\, 	\mathrm d  y
		}{
		\int_v^\infty 
		% 
			e^{  - \frac{(w-v)^2}{2t}  } 
		\frac{ (w-v) }{ t \sqrt{2 \pi t } }
		e^{  - \frac{\mu^2 t}{2} + \mu ( w - v)   } \,  \mathrm d  w
	} 
	\\
	%
	%
	%
	&=
	\int_v^x \sum_{k = - \infty}^{+\infty}
	% 
		e^{    -   \frac{(y - v - 2k(x-v))^2}{2 s} } 
	\frac { (y - v - 2k (x-v) )}{s\sqrt{2 \pi s }}
	e^{ -2 k \mu (x-v)}
	\, \times 
	\\
	& \qquad \times 
	\frac{ 
		\int_v^\infty
		\left[
		%
			e^{  - \frac{(w - y )^2}{  2 (t-s) }    }
			- 
			e^{  - \frac{  (w + y - 2 v)^2}{ 2 (t-s) }    } 
			\right]
		%
	e^{ \mu w} \, \frac{ \mathrm d w}{\sqrt{2 \pi (t-s)} }
%		
		\,\mathrm d y
	}{
		\int_v^\infty 
		% 
			e^{  - \frac{(w-v)^2}{2t}  } 
		\frac { (w-v) }{t \sqrt{2 \pi t } } 
		e^{ \mu w   } \,  \mathrm d w
	} \, .
\end{align*}
%
%
%
Formula \eqref{eq:max-bmd-t} for $  u \downarrow v $ leads to 
%
\begin{align*}
		&
		P\bigg\{ \max_{0 \leq z \leq t} B^\mu(z) <x \Big |  \inf_{0 < z < t} B^\mu (z) > v, B^\mu(0) = v  \bigg\}
		\numberthis 
		\label{eq:max-bmd-t-v}
		\\
		&=
		\frac{  
		\sum_{k = -\infty} ^ { + \infty}
		e^{  - 2 \mu k (x-v)  }
		\int_v^x
			e^ {   -  \frac{(y - v - 2k(x-v))^2}{2t}  }
			(y - v - 2k ( x-v) )
			e^{ \mu y } \, \mathrm d y
		}{
		\int_v^\infty 
		e^{  - \frac{(y - v)^2}{2t}  } (y-v) 
		e^{ \mu y } \,\mathrm d y	
		      }
	    \\
	    %
	    %
	    %
	    &=
	    \frac{  
	    	\sum_{k = -\infty} ^ { + \infty}
	    	e^{  - 2 \mu k (x-v)  }
	    	\int_0^{x-v}
	    	e^ {   -  \frac{(w  - 2k(x-v))^2}{2t}  }
	    	(w- 2k ( x-v) )
	    	e^{ \mu w } \, \mathrm d w
	    }{
	    	t[1 + \mu \int_0^\infty 
	    	e^{  - \frac{y^2}{2t}  } 
	    	e^{ \mu y } \,\mathrm d y]	
	    } \, .
\end{align*}
%
%
%
Observe that the passage to the limit fo $ u \downarrow v $ is justified by \autoref*{thm:weak-conv-mdr} and by the continuous mapping theorem as observed
in Section 2.  For $ v=0 $ result \eqref{eq:max-bmd-t-v} further simplifies as 
%
\begin{align*}
&
P\bigg\{ \max_{0 \leq z \leq t} B^\mu(z) <x \Big |  \inf_{0 < z < t} B^\mu (z) > 0, B^\mu(0) = 0  \bigg\}
\numberthis 
\label{eq:max-bmd-t-v0}
\\
&=
\frac{  
	\sum_{k = -\infty} ^ { + \infty}
	e^{  - 2 \mu k x  }
	\int_0^{x}
	e^ {   -  \frac{(w  - 2kx)^2}{2t}  }
	(w- 2kx )
	e^{ \mu w } \, \mathrm d w
}{
	t[ 1 + \mu \int_0^\infty 
	e^{  - \frac{y^2}{2t}  } 
	e^{ \mu y } \,\mathrm d y	]
}
\\
%
%
&=
%
\frac{  
	\sum_{r = -\infty} ^ { + \infty}
	(-1)^r
	e^{  -  \mu r x - \frac{x^2 r^2}{2t}  } 
	+ \mu
	\sum_{r = -\infty}^{+ \infty}
	\int_{- 2 rx}^{x - 2 r x }
	e^ {   -  \frac{w ^2}{2t}  + \mu w}
 \, \mathrm d w
}{
	1 + \mu \int_0^\infty 
	e^{  - \frac{y^2}{2t}  } 
	e^{ \mu y } \,\mathrm d y	
} \, \, .
\end{align*}
%
%
Formula \eqref{eq:max-bmd-t-v0} can be written in a more convenient way by observing that 
%
%
\begin{align*}
	\sum_{r=-\infty}^{+ \infty } 
	\int_{- 2 r x } ^ { x - 2 r x } 
	e^ {   -  \frac{w ^2}{2t}  + \mu w}
	\, \mathrm d w 
	&=
	\sum_{  r = 0 } ^ {+ \infty}  
	\int_{ 2 r x } ^ { x + 2 r x } 
	e^ {   -  \frac{w ^2}{2t}  + \mu w}
	\, \mathrm d w 
	+ 
	\sum_{  r = 1 } ^ {+ \infty}  
	\int_{-  2 r x } ^ { x  -  2 r x } 
	e^ {   -  \frac{w ^2}{2t}  + \mu w}
	\, \mathrm d w 
	\\
	%
	%
	&=
	\int_0^\infty e^{ - \frac{w^2}{2t} } g (w, x) \,\mathrm d w 
	\\
%	&=
%	\int_0^\infty e^{ - \frac{w^2}{2t} } e^{ \mu w (-1)^{ \left \lfloor \frac w x \right \rfloor} } \,\mathrm d w
\end{align*}
%
where 
\begin{align*}
g(w, x)
&= e^{ \mu w (-1)^{ \left \lfloor \frac w x \right \rfloor} }
\end{align*}
and $  \left \lfloor  z \right \rfloor  $ denotes the integer part of the real number $ z $.
%
%
In conclusion
\begin{align*}
&
P\bigg\{ \max_{0 \leq z \leq t} B^\mu(z) <x \Big |  \inf_{0 < z < t} B^\mu (z) > 0, B^\mu(0) = 0  \bigg\}
\label{eq:max-bmd-t-v0-fin}
\numberthis
\\
&=
\frac{  
	\sum_{r = -\infty} ^ { + \infty}
	(-1)^r
	e^{  -  \mu r x - \frac{x^2 r^2}{2t}  } 
	+ \mu
	\int_0^\infty e^{ - \frac{w^2}{2t} } e^{ \mu w (-1)^{ \left \lfloor \frac w x \right \rfloor} } \,\mathrm d w
}{
	1 + \mu \int_0^\infty 
	e^{  - \frac{y^2}{2t}  } 
	e^{ \mu y } \,\mathrm d y	
} \,\, .
\end{align*}
%
%
Observe that  
\begin{enumerate}[(i)]
\item for $ \mu = 0 $ we obtain the well-known distribution of the driftless meander
%
\begin{equation}\label{eq:max-bmd-mu0}
P\bigg\{ \max_{0 \leq z \leq t} B(z) <x \Big |  \inf_{0 < z < t} B (z) > 0, B(0) = 0  \bigg\}
=
\sum_{r = - \infty} ^ { + \infty} 
(-1)^r
e^{  - \frac{x^2 r^2 }{2t}  } \,\, .
\end{equation}
%
\item 
For $  x \to \infty  $, $  \mu \neq 0 $, we obtain that  \eqref{eq:max-bmd-t-v0-fin} tends to 1
as can be seen from \eqref{eq:max-bmd-t-v}.
%
\item 
In order to prove that \eqref{eq:max-bmd-t-v0-fin} for $  x \to 0  $, $  \mu \neq 0 $ 
we write 
\[
\sum_{k=-\infty}^{+ \infty} (-1)^k e^{- \frac{x^2 k^2}{2t} + \mu k x } 
= 
\sum_{k=-\infty}^{+ \infty} (-1)^k e^{- \frac{x^2 k^2}{2t} } 
\left(
1 + \int_0^{\mu k x} e^w \, \mathrm d w 
\right). 
\]
The first term tends to zero because we can apply
%
\[
\sum_{k=-\infty}^{+ \infty} (-1)^k e^{- \frac{x^2 k^2}{2t} } 
= 
\frac{\sqrt{4 \pi t}}{x} 
\sum_{k=1}^{+ \infty} e^{- \frac{ (2k-1)^2 \pi^2 t }{4 x^2} } 
\]
(see \cite{durbin}, eq. (3.4.9)).
%
\item 
Note that for $  \mu = 0 $ we have that  \eqref{eq:max-bmd-mu0} coincides with the
distribution of the maximum of the Brownian bridge, that is
\begin{equation*}
P\bigg\{ \max_{0 \leq z \leq t} B(z) <x \Big |  \inf_{0 < z < t} B (z) > 0, B(0) = 0  \bigg\}
= 
P\bigg\{ \max_{0 \leq z \leq t} |B(z)| < \frac x2 \Big |  B(0) = 0, B(t) = 0  \bigg\} \,\, .
\end{equation*}
\end{enumerate}


%


%

\subsection{First passage times.}
We now study the distribution of the first passage time of a Brownian motion
 evolving 
under the condition that the minimum of the process is larger than $ v $ (eventually $ v=0 $) up to time $ t > 0$,
the process being free afterwards.
The first passage time is denoted  by $ T_x = \inf \{s < t' : B^\mu(s) = x\} $, $ t'>t $. 

%
For $ s <  t $ we infer  from \eqref{eq:max-bmd-ini}  that 
%
%
\begin{align*}
	&
	P\left\{ T_x > s \Big| \min_{ 0 \leq z \leq t }B^\mu( z) > v, B^\mu(0) = u \right\} 
	\numberthis \label{eq:first-psg-dist}
	\\
	&=
	\int_v^x P\left\{ \max_{ 0 \leq z \leq s }B^\mu( z) < x, \min_{ 0 \leq z \leq s }B^\mu( z) > v , 
	B^\mu ( s ) \in \mathrm d y  \Big | B^\mu ( 0) = u \right\}	\times 
	\\
	& \qquad \times 
	\frac{
		P\left\{  \min_{ s \leq z \leq t }B^\mu( z) > v \Big | B^\mu ( s) = y \right\}			
	}{
		P\left\{  \min_{ 0 \leq z \leq t }B^\mu( z) > v \Big | B^\mu ( 0) = u \right\}
	}
	\\
	&=
	\int_v^x \, \frac{\mathrm d y}{\sqrt{2 \pi s}} \sum_{k = - \infty}^{+\infty}
	\left[ 
	%
	e^{    -   \frac{(y - u - 2k(x-v))^2}{2s} } 
	- 
	%
	e^{    -   \frac{(2v - y - u +2k(x-v))^2}{2s} }  
	\right ] 
	e^{ - \frac{\mu^2s}{2} + \mu ( y - u - 2k(x-v))} 
	\,\,\times 
	\\
	& \qquad \times 
	%
	\frac{
		P\Big\{   \min_{s \leq z \leq t} B^\mu(z)   > v  \Big | B^\mu ( s) = y \Big\}
	}{
		\int_v^\infty 
		\left[ 
		% 
		e^{  - \frac{(w-u)^2}{2t}  } 
		- 
		%
		e^{  - \frac{(2v - w-u)^2}{2t}  } 
		\right]
		e^{  - \frac{\mu^2 t}{2} + \mu ( w - u)   } \, \frac{ \mathrm d w}{\sqrt{2 \pi t} } 
	}
\end{align*}
for $ x > v$. If $ s > t $ we have that
\begin{align*}
&
	P\left\{ T_x \in \mathrm d s \Big| \min_{ 0 \leq z \leq t }B^\mu( z) > v, B^\mu(0) = u \right\} 
	/ \mathrm d s
	\numberthis \label{eq:first-psg-dist-ts}
	\\
	&=
	%
	\int_v^x 
	P\left\{ T_x\in \mathrm d s \Big| B^\mu(t) = y \right\} / \mathrm d s
	\,\,
	P\left\{  
	B^\mu(t) \in \mathrm d y, \max_{0 \leq z \leq t} B^\mu (z) < x \Big| \min_{ 0 \leq z \leq t } B^\mu(z) > v , B^\mu(0) = u
	\right\}
	\\
	&=
	%
	\frac{
		\int_v^x
		\frac{ (x-y)\, e^{ - \frac{  |x- y - \mu (s-t)|^2} {2(s-t)} } }
		{\sqrt{2 \pi (s-t)^3} } 
		%
		\sum_{k = - \infty}^{+\infty}
		\left[ 
		%
		e^{    -   \frac{(y - u - 2k(x-v))^2}{2t} } 
		- 
		%
		e^{    -   \frac{(2v - y - u +2k(x-v))^2}{2t} }  
		\right ] 
		%
			e^{  \mu ( y  - 2k(x-v))}
		%
		%
		 \, \mathrm d y}
	{\int_v^\infty \left(  e^{- \frac{(w - u)^2}{2t}} -  e^{- \frac{(2v - w - u)^2}{2t}}  \right)
	e^{\mu w} \, \mathrm d w 
	} \,\, .
	%
\end{align*}
%
% Clearly 
%\begin{align*} 
%	&
%	m(t;s,y) = 
% 	P\Big\{   \min_{s \leq z \leq t} B^\mu(z)   > v  \Big | B^\mu ( s) = y \Big\}
% 	\\
% 	&=
% 	\int_v^\infty 
% 	\left[ 
% 	% 
% 	e^{  - \frac{(w-y)^2}{2(t-s)}  } 
% 	- 
% 	%
% 	e^{  - \frac{(2v - w-y)^2}{2(t-s)}  } 
% 	\right]
% 	e^{  - \frac{\mu^2 (t-s)}{2} + \mu ( w - y) }  \frac{\mathrm d w}{\sqrt{2\pi(t-s)}}
%\end{align*}
%
For  $  u \to v $ and $ s < t $ the first-passage time becomes
%
%
\begin{align*}
&
	P\left\{ T_x > s \Big| \min_{ 0 \leq z \leq t }B^\mu( z) > v, B^\mu(0) = v \right\} =
	\numberthis \label{eq:first-psg-dist-v}
	\\
	&=
		\frac{ 
	\int_v^x \sum_{k = - \infty}^{+\infty}
	% 
	e^{    -   \frac{(y - v - 2k(x-v))^2}{2 s} } 
	\frac { (y - v - 2k (x-v) )}{s\sqrt{2 \pi s }}
	e^{ - \frac {\mu^2 s } 2 + \mu( y-v - 2 k \mu (x-v) ) }
	\,   
%	\\
%	& \qquad \times 
%
		%
		m(t;s,y) \,\mathrm d y
	}{
		\int_v^\infty 
		% 
		e^{  - \frac{(w-v)^2}{2t}  } 
		%
		\frac{ (w-v)  }{\sqrt{2 \pi t} }
		e^{ \mu (w-v) + \frac{\mu^2 t}{2}   } \,  \mathrm d w
	} \,\,
\end{align*}
%
%
where 
%

\begin{align*} 
	&
	m(t;s,y) = 
 	P\Big\{   \min_{s \leq z \leq t} B^\mu(z)   > v  \Big | B^\mu ( s) = y \Big\}
 	\numberthis \\
 	&=
 	\int_v^\infty 
 	\left[ 
 	% 
 	e^{  - \frac{(w-y)^2}{2(t-s)}  } 
 	- 
 	%
 	e^{  - \frac{(2v - w-y)^2}{2(t-s)}  } 
 	\right]
 	e^{  - \frac{\mu^2 (t-s)}{2} + \mu ( w - y) }  \frac{\mathrm d w}{\sqrt{2\pi(t-s)}} \,\, .
\end{align*}


%
In the case $  t < s< t' $, the limit for $ u \downarrow v $ in 
\eqref{eq:first-psg-dist-ts}
yields
%
\begin{align*}
&
P\left\{ T_x \in \mathrm d s \Big| \inf_{ 0 < z < t }B^\mu( z) > v, B^\mu(0) = v \right\} 
/ \mathrm d s
\numberthis \label{eq:first-psg-dist-ts-v}
\\
%
&=
\frac{\int_v^x 
	%
	\frac{ x-y}
	{\sqrt{2 \pi (s-t)^3} } 
	e^{ - \frac{  |x- y - \mu (s-t)|^2} {2(s-t)} }
	\sum_{k = - \infty}^{+\infty}
	(y - v - 2k(x-v))
	e^{    -   \frac{(y - v - 2k(x-v))^2}{2t} } 
	%
	e^{  \mu ( y  - 2k(x-v))}
	%
	%
	\, \mathrm d y}
{
	\int_0^\infty 
	(w-v) e^{- \frac{ (w - v)^2} { 2 t } + \mu w }  
	\, \mathrm d w
}\,\,.
\end{align*}
%
%
Some further simplification can be obtained in  \eqref{eq:first-psg-dist-v} and \eqref{eq:first-psg-dist-ts-v}
for $ v=0 $. For $ s < t  $ we have in particular that \eqref{eq:first-psg-dist-v}
further simplifies as 
\begin{align*}
&
P\left\{ T_x > s \Big| \inf_{ 0 < z < t }B^\mu( z) > 0, B^\mu(0) = 0 \right\} 
\numberthis \label{eq:first-psg-dist-0}
\\
&=
\int_0^x \sum_{k = - \infty}^{+\infty}
% 
e^{    -   \frac{(y  - 2kx)^2}{2 s} } 
\frac { (y -  2k x )}{s\sqrt{2 \pi s }}
e^{ -2 k \mu x}
\,   \mathrm d y
%
\frac{ 
	\int_0^\infty
	\left[
	%
	e^{  - \frac{(w - y )^2}{  2 (t-s) }    }
	- 
	e^{  - \frac{  (w + y )^2}{ 2 (t-s) }    } \right]
	%
	\, \frac{ e^{ \mu w}  }{\sqrt{2 \pi (t-s)} }
	 \mathrm d w
	%
}{
	\int_0^\infty 
	% 
	\frac w {t \sqrt{2 \pi t} }
	e^{  - \frac{w^2}{2t} + \mu w   } 	 
	\mathrm d w
} \,\,  .
\end{align*}











% !TeX root = ./mdr-main.tex